Slightly more interesting files

VCV-io/OracleComp/OracleComp.lean
@@ -5,36 +5,30 @@ Authors: Devon Tuma
 -/
 import «VCV-io».OracleComp.OracleSpec
 
-open OracleSpec
-
 inductive OracleComp (spec : OracleSpec) : Type → Type 1
-  | pure' (α : Type) (a : α) : OracleComp spec α
-  | query_bind' (i : spec.ι) (t : spec.domain i) (α : Type)
-      (oa : spec.range i → OracleComp spec α) : OracleComp spec α
+| pure' (α : Type) (a : α) : OracleComp spec α
+| query_bind' (i : spec.ι) (t : spec.domain i) (α : Type)
+    (oa : spec.range i → OracleComp spec α) : OracleComp spec α
 
 namespace OracleComp
 
-variable {spec : OracleSpec} {α β γ : Type}
-
-def default_result : {α : Type} → OracleComp spec α → α
-  | _, pure' α a => a
-  | _, query_bind' _ _ α oa => default_result (oa default)
+def defaultResult {spec : OracleSpec} : {α : Type} → OracleComp spec α → α
+| _, pure' α a => a
+| _, query_bind' _ _ α oa => defaultResult (oa default)
 
 instance (spec : OracleSpec) (α : Type) [h : Nonempty α] :
   Nonempty (OracleComp spec α) := h.elim (λ x ↦ ⟨pure' α x⟩)
-
 instance (spec : OracleSpec) (α : Type) [Inhabited α] :
   Inhabited (OracleComp spec α) := ⟨pure' α default⟩
-
 instance (spec : OracleSpec) (α : Type) [h : IsEmpty α] :
-  IsEmpty (OracleComp spec α) := ⟨λ oa ↦ h.1 (default_result oa)⟩
+  IsEmpty (OracleComp spec α) := ⟨λ oa ↦ h.1 (defaultResult oa)⟩
 
-def base_inhabited (oa : OracleComp spec α) : Inhabited α := ⟨oa.default_result⟩
+variable {spec : OracleSpec} {α : Type}
+
+def baseInhabited (oa : OracleComp spec α) : Inhabited α := ⟨oa.defaultResult⟩
 
 section Monad
 
-/-- We define a monadic bind operation on `oracle_comp` by induction on the first computation.
-With this definition `oracle_comp` satisfies the monad laws (see `oracle_comp.is_lawful_monad`). -/
 def bind' : (α β : Type) → OracleComp spec α → (α → OracleComp spec β) → OracleComp spec β
 | _, _, pure' α a, ob => ob a
 | _, β, query_bind' i t α oa, ob => query_bind' i t β (λ u ↦ bind' α β (oa u) ob)
@@ -42,54 +36,21 @@ def bind' : (α β : Type) → OracleComp spec α → (α → OracleComp spec β
 instance (spec : OracleSpec) : Monad (OracleComp spec) :=
 { pure := @pure' spec, bind := @bind' spec }
 
-protected lemma pure_def (spec : OracleSpec) {α : Type} (a : α) :
-  (pure a : OracleComp spec α) = pure' α a := rfl
+@[simp] protected lemma pure'_eq_pure (spec : OracleSpec) (a : α) :
+  pure' α a = (pure a : OracleComp spec α) := rfl
 
-protected lemma bind_def {spec : OracleSpec} {α β : Type}
-  (oa : OracleComp spec α) (ob : α → OracleComp spec β) :
-  oa >>= ob = bind' α β oa ob := rfl
+@[simp] protected lemma bind'_eq_bind (oa : OracleComp spec α) (ob : α → OracleComp spec β) :
+  bind' α β oa ob = oa >>= ob := rfl
 
 instance (spec : OracleSpec) : LawfulMonad (OracleComp spec) :=
 LawfulMonad.mk' _
   (λ oa ↦ by
-    induction' oa with α a i t α oa hoa
-    · rfl
+    induction' oa with α a i t α oa hoa; · rfl
     · exact congr_arg (query_bind' i t α) (funext (λ u ↦ hoa u)))
   (λ x ob ↦ rfl)
   (λ oa ob oc ↦ by
-    induction' oa with α a i t α oa hoa
-    · rfl
-    · refine congr_arg (query_bind' i t _) <| funext (λ u ↦ hoa u ob))
-
--- @[simp] protected lemma pure'_eq_return (spec) :
---   (pure' α : α → oracle_comp spec α) = return := funext (λ a ↦ rfl)
-
--- @[simp] protected lemma pure_eq_return (spec) :
---   (pure : α → oracle_comp spec α) = return := funext (λ a, rfl)
-
--- @[simp] protected lemma bind'_eq_bind (spec) :
---   (bind' α β : oracle_comp spec α → (α → oracle_comp spec β) → oracle_comp spec β) = (>>=) := rfl
-
--- protected lemma bind_return_comp_eq_map (oa : OracleComp spec α) (f : α → β) :
---   oa >>= pure ∘ f = f <$> oa := rfl
-
--- protected lemma map_eq_bind_return_comp (oa : oracle_comp spec α) (f : α → β) :
---   f <$> oa = oa >>= return ∘ f := rfl
-
--- protected lemma return_bind (a : α) (ob : α → oracle_comp spec β) :
---   return a >>= ob = ob a := pure_bind a ob
-
--- protected lemma bind_return (oa : oracle_comp spec α) : oa >>= return = oa := bind_pure oa
-
--- @[simp] lemma bind_query_bind' (i : spec.ι) (t : spec.domain i)
---   (oa : spec.range i → oracle_comp spec α) (ob : α → oracle_comp spec β) :
---   (query_bind' i t α oa) >>= ob = query_bind' i t β (λ u, oa u >>= ob) := rfl
-
--- @[simp] lemma map_map_eq_map_comp (oa : oracle_comp spec α) (f : α → β) (g : β → γ) :
---   g <$> (f <$> oa) = (g ∘ f) <$> oa :=
--- by simp [oracle_comp.map_eq_bind_return_comp, bind_assoc]
-
--- lemma map_return (f : α → β) (a : α) : f <$> (return a : OracleComp spec α) = return (f a) := rfl
+    induction' oa with α a i t α oa hoa; · rfl
+    · exact congr_arg (query_bind' i t _) <| funext (λ u ↦ hoa u ob))
 
 protected lemma bind_congr {oa oa' : OracleComp spec α} {ob ob' : α → OracleComp spec β}
   (h : oa = oa') (h' : ∀ x, ob x = ob' x) : oa >>= ob = oa' >>= ob' :=
@@ -99,16 +60,8 @@ lemma ite_bind (p : Prop) [Decidable p] (oa oa' : OracleComp spec α)
   (ob : α → OracleComp spec β) : ite p oa oa' >>= ob = ite p (oa >>= ob) (oa' >>= ob) :=
 by split_ifs <;> rfl
 
--- lemma bind_seq (oa : OracleComp spec α) (og : OracleComp spec (α → β))
---   (oc : β → OracleComp spec γ) : (og <*> oa) >>= oc = og >>= λ f ↦ oa >>= (oc ∘ f) :=
--- by simp [seq_eq_bind_map, map_eq_bind_pure_comp, bind_assoc]
-
 end Monad
 
-section query
-
-/-- Shorthand for running a query and returning the value.
-Generally this should be preferred over using `query_bind'` directly. -/
 def query (i : spec.ι) (t : spec.domain i) : OracleComp spec (spec.range i) :=
 query_bind' i t (spec.range i) (pure' (spec.range i))
 
@@ -119,9 +72,70 @@ lemma query_def (i : spec.ι) (t : spec.domain i) :
   (t : spec.domain i) (oa : spec.range i → OracleComp spec α) :
   query_bind' i t α oa = query i t >>= oa := rfl
 
-@[reducible, inline] def coin : OracleComp coinSpec Bool :=
-query (spec := coinSpec) () ()
+@[reducible, inline] def coin : OracleComp OracleSpec.coinSpec Bool :=
+query (spec := OracleSpec.coinSpec) () ()
+variable (C : Nat → Type u)
 
-end query
+protected def induction_on {spec : OracleSpec}
+  {C : Π {α : Type}, OracleComp spec α → Prop}
+  (h_pure : ∀ {α : Type} (a : α), C (pure a))
+  (h_query_bind : ∀ (i : spec.ι) (t : spec.domain i) {α : Type}
+    (oa : spec.range i → OracleComp spec α),
+    (∀ u, C (oa u)) → C (query i t >>= oa)) :
+  {α : Type} → (oa : OracleComp spec α) → C oa
+| _, (pure' α a) => h_pure a
+| _, (query_bind' i t α oa) => h_query_bind i t oa
+  (λ u ↦ OracleComp.induction_on h_pure h_query_bind (oa u))
+
+@[simp] lemma pure_inj (x x' : α) :
+  (pure x : OracleComp spec α) = (pure x' : OracleComp spec α) ↔ x = x' :=
+⟨λ h ↦ OracleComp.noConfusion h (λ _ hx ↦ eq_of_heq hx), λ h ↦ h ▸ rfl⟩
+
+@[simp] lemma query_inj (i : spec.ι) (t t' : spec.domain i) :
+  query i t = query i t' ↔ t = t' :=
+⟨λ h ↦ OracleComp.noConfusion h (λ _ ht _ _ ↦ eq_of_heq ht), λ h ↦ h ▸ rfl⟩
+
+@[simp] lemma query_bind_inj (i i' : spec.ι) (t : spec.domain i) (t' : spec.domain i')
+  (oa : spec.range i → OracleComp spec α) (oa' : spec.range i' → OracleComp spec α) :
+  query i t >>= oa = query i' t' >>= oa' ↔ ∃ h : i = i', h ▸ t = t' ∧ h ▸ oa = oa' := by
+  sorry
+
+@[simp] lemma pure_ne_query (i : spec.ι) (t : spec.domain i) (u : spec.range i) :
+  pure u ≠ query i t := OracleComp.noConfusion
+
+@[simp] lemma query_ne_pure (i : spec.ι) (t : spec.domain i) (u : spec.range i) :
+  query i t ≠ pure u := OracleComp.noConfusion
+
+@[simp] lemma pure_ne_query_bind (x : α) (i : spec.ι) (t : spec.domain i)
+  (oa : spec.range i → OracleComp spec α) : pure x ≠ query i t >>= oa := OracleComp.noConfusion
+
+@[simp] lemma query_bind_ne_pure (i : spec.ι) (t : spec.domain i)
+  (oa : spec.range i → OracleComp spec α) : query i t >>= oa ≠ (pure x) := OracleComp.noConfusion
+
+@[simp] lemma bind_eq_pure_iff (oa : OracleComp spec α) (ob : α → OracleComp spec β) (y : β) :
+  oa >>= ob = pure y ↔ ∃ x : α, oa = pure x ∧ ob x = pure y := by
+  refine ⟨λ h ↦ ?_, λ h ↦ ?_⟩
+  · match oa with
+    | pure' _ x => exact ⟨x, rfl, h⟩
+    | query_bind' i t _ oa => simp at h
+  · obtain ⟨x, hxa, hxb⟩ := h
+    rw [hxa, pure_bind, hxb]
+
+@[simp] lemma pure_eq_bind_iff (y : β) (oa : OracleComp spec α) (ob : α → OracleComp spec β) :
+  pure y = oa >>= ob ↔ ∃ x : α, oa = pure x ∧ ob x = pure y :=
+eq_comm.trans (bind_eq_pure_iff oa ob y)
+
+protected instance decidableEq {α : Type} [h : DecidableEq α] : DecidableEq (OracleComp spec α)
+| pure' _ x, pure' _ x' => by simpa [pure_inj x x'] using h x x'
+| pure' _ x, query_bind' i t _ oa => by simpa using Decidable.isFalse not_false
+| query_bind' i t _ oa, pure' _ x => by simpa using Decidable.isFalse not_false
+| query_bind' i t _ oa, query_bind' i' t' _ oa' => by
+  by_cases hi : i = i'
+  · induction hi; simp
+    suffices Decidable (oa = oa') from inferInstance
+    suffices Decidable (∀ u, oa u = oa' u) from decidable_of_iff' _ Function.funext_iff
+    suffices ∀ u, Decidable (oa u = oa' u) from Fintype.decidableForallFintype
+    exact λ u ↦ OracleComp.decidableEq (oa u) (oa' u)
+  · simpa [hi] using Decidable.isFalse not_false
 
 end OracleComp
